Reflecting at home changes I made at school.

Modal/cpl/proof.lean
@@ -1,34 +1,48 @@
-/- I do not care how the proof system is defined, as long
-as it satisfies the needed metatheorems. -/
+/- I do not care how the proof system is defined,
+as long as it satisfies the needed metatheorems. -/
 
 
 import Modal.cpl.syntax
+import Mathlib.Data.Set.Defs
 
 namespace CPL
 
-def CPLProof {Form : Type} [CPLSyntax Form] (A : Form) : Prop := by
+def has_proof {𝓕 : Type} [Syntax 𝓕] (Γ : Set 𝓕) (φ : 𝓕) : Prop := by
   admit
 
+notation:50 Γ " ⊢ " φ => has_proof Γ φ
+notation:50 "⊢ " φ => has_proof ∅ φ
 
-variable {Form : Type} [CPLSyntax Form]
+variable {𝓕 : Type} [Syntax 𝓕]
 
 -- A valuation is a function from formulas to propositions that respects
 -- the classical propositional connectives.
 -- So we need to say what the valuation function is, and prove
 -- that it respects ⊥ and → (the basic connectives).
-structure Valuation (Form : Type) [CPLSyntax Form] where
-  eval : Form → Prop
+-- A valuation is the concept of model in CPL.
+structure Valuation (𝓕 : Type) [Syntax 𝓕] where
+  eval : 𝓕 → Prop
   eval_bot : eval ⊥ = False
   eval_impl : ∀ φ ψ, eval (φ → ψ) = (eval φ → eval ψ)
 
-notation:50 v " ⊨ " φ => Valuation.eval v φ
+def models_set (v : Valuation 𝓕) (Γ : Set 𝓕) : Prop :=
+  ∀ ψ, ψ ∈ Γ → v.eval ψ
 
-def is_tautology (φ : Form) : Prop :=
-  ∀ (v : Valuation Form), v ⊨ φ
+def semantic_consequence (Γ : Set 𝓕) (φ : 𝓕) : Prop :=
+  ∀ (v : Valuation 𝓕), models_set v Γ → v.eval φ
+
+notation:50 Γ " ⊨ " φ => semantic_consequence Γ φ
+
+-- that is, is a tautology
+def is_valid (φ : 𝓕) : Prop :=
+  ∀ (v : Valuation 𝓕), v.eval φ
 
 -- provable formulas are tautologies
 -- The proof of this would depend on how the CPL proof system is defined.
-theorem cpl_sound : ∀ {φ : Form}, CPLProof φ → is_tautology φ := by
+theorem cpl_sound_weak : ∀ {φ : 𝓕}, (∅ ⊢ φ) → (∅ ⊨ φ) := by
+  admit
+
+theorem cpl_sound_strong : ∀ {Γ : Set 𝓕} {φ : 𝓕}, (Γ ⊢ φ) → (Γ ⊨ φ) := by
   admit
 
 end CPL
