Modal/modal/formula.lean
@@ -1,23 +1,27 @@
-/- As in the classical case, we define the syntax and the formulas separately.
+/- We define the syntax and the formulas separately.
 This would be especially useful if we intend to work with products of logics
 later on, in which each logic would need to use different actual modal
-operators. -/
+operators.
+
+𝓐 (backslash MCA) represent the type of atoms (= atomic propositions
+= propositional variables). Typically, 𝓐 = ℕ or 𝓐 = String, but also
+uncountable types are possible, e.g. 𝓐 = ℝ. -/
 
 
 import Modal.modal.syntax
 
-namespace ModalFormula
+namespace Modal
 
-inductive ModalFormula (α : Type) where
-  | atom : α → ModalFormula α
-  | bot  : ModalFormula α
-  | impl : ModalFormula α → ModalFormula α → ModalFormula α
-  | box  : ModalFormula α → ModalFormula α
+inductive Formula (𝓐 : Type) where
+  | atom : 𝓐 → Formula 𝓐
+  | bot  : Formula 𝓐
+  | impl : Formula 𝓐 → Formula 𝓐 → Formula 𝓐
+  | box  : Formula 𝓐 → Formula 𝓐
 deriving DecidableEq
 
-instance (α : Type) : ModalSyntax (ModalFormula α) where
-  bot  := ModalFormula.bot
-  impl := ModalFormula.impl
-  box  := ModalFormula.box
+instance (𝓐 : Type) : Syntax (Formula 𝓐) where
+  bot  := Formula.bot
+  impl := Formula.impl
+  box  := Formula.box
 
-end ModalFormula
+end Modal
