Modal/modal/logics/logic_E.lean
@@ -3,11 +3,11 @@ import Modal.modal.formula
 import Modal.modal.axioms_rules
 
 
-open ModalAxioms ModalRules CPL ModalFormula
+open Modal.Axioms Modal.Rules
 
-variable {α : Type} [ModalSyntax α]
+variable {α : Type}
 
-inductive EProof : ModalFormula α → Prop where
-  | cpl {p : ModalFormula α} (h_cpl : CPLProof p) : EProof p
-  | rl_re {p q : ModalFormula α} (h_prem : EProof (rl_re p q).premise) :
-                                           EProof (rl_re p q).conclusion
+inductive EProof : Modal.Formula α → Prop where
+  | cpl {p : Modal.Formula α} (h_cpl : CPL.has_proof ∅ p) : EProof p
+  | rl_re {p q : Modal.Formula α} (h_prem : EProof (rl_re p q).premise) :
+                                            EProof (rl_re p q).conclusion
