Modal/modal/logics/logic_K.lean
@@ -3,14 +3,14 @@ import Modal.modal.formula
 import Modal.modal.axioms_rules
 
 
-open ModalAxioms ModalRules CPL ModalFormula
+open Modal.Axioms Modal.Rules
 
-variable {α : Type} [ModalSyntax α]
+variable {α : Type}
 
-inductive KProof : ModalFormula α → Prop where
-  | classical {p : ModalFormula α} (h : CPLProof p) : KProof p
-  | rl_re {p q : ModalFormula α} (h : KProof (rl_re p q).premise) :
-                                      KProof (rl_re p q).conclusion
-  | rl_nec {p : ModalFormula α} (h : KProof (rl_nec p).premise) :
-                                     KProof (rl_nec p).conclusion
-  | ax_k {p q : ModalFormula α} : KProof (ax_k p q)
+inductive KProof : Modal.Formula α → Prop where
+  | classical {p : Modal.Formula α} (h : CPL.has_proof ∅ p) : KProof p
+  | rl_re {p q : Modal.Formula α} (h : KProof (rl_re p q).premise) :
+                                       KProof (rl_re p q).conclusion
+  | rl_nec {p : Modal.Formula α} (h : KProof (rl_nec p).premise) :
+                                      KProof (rl_nec p).conclusion
+  | ax_k {p q : Modal.Formula α} : KProof (ax_k p q)
