Modal/modal/models/nbhd.lean
@@ -5,7 +5,7 @@ import Modal.modal.formula
 
 namespace Neighborhood
 
-open CPL ModalFormula
+open CPL
 
 
 structure Frame where
@@ -24,26 +24,26 @@ class IsUpwardClosed (f : Frame) : Prop where
 variable {α : Type}
 
 -- Defines truth at a specific world w, that is m, w ⊨ φ.
-def world_sat (m : Model α) (w : m.frame.world) : ModalFormula α → Prop
+def world_sat (m : Model α) (w : m.frame.world) : Modal.Formula α → Prop
   | .atom a   => m.val w a
   | .bot      => False
   | .impl φ ψ => world_sat m w φ → world_sat m w ψ
   | .box φ    => {v | world_sat m v φ} ∈ m.frame.nbhd w
 
 -- Defines truth in an entire model m, that is m ⊨ φ.
-def model_sat (m : Model α) (φ : ModalFormula α) : Prop :=
+def model_sat (m : Model α) (φ : Modal.Formula α) : Prop :=
   ∀ w, world_sat m w φ
 
 -- Defines truth in an entire frame f, that is f ⊨ φ.
-def frame_sat (f : Frame) (φ : ModalFormula α) : Prop :=
+def frame_sat (f : Frame) (φ : Modal.Formula α) : Prop :=
   ∀ val, model_sat ⟨f, val⟩ φ
 
 -- Defines truth in all possible models, that is ⊨ φ.
-def valid (φ : ModalFormula α) : Prop :=
+def valid (φ : Modal.Formula α) : Prop :=
   ∀ (f : Frame), frame_sat f φ
 
 -- Defines truth in all frames satisfying a given class/property.
-def valid_in_class (P : Frame → Prop) (φ : ModalFormula α) : Prop :=
+def valid_in_class (P : Frame → Prop) (φ : Modal.Formula α) : Prop :=
   ∀ (f : Frame), P f → frame_sat f φ
 
 end Neighborhood
