Modal/modal/sound_complete/logicE_nbhd.lean
@@ -3,13 +3,10 @@ import Modal.modal.models.nbhd
 import Modal.modal.logics.logic_E
 
 
-open ModalFormula
-
-
 variable {α : Type}
 
 -- Soundness and completeness of logic E with respect to neighborhood models
 -- Well-known result
 theorem logicE_nbhd_sc :
-    ∀ (φ : ModalFormula α), Neighborhood.valid φ ↔ EProof φ := by
+    ∀ (φ : Modal.Formula α), Neighborhood.valid φ ↔ EProof φ := by
     admit
