Modal/modal/sound_complete/logicK_kripke.lean
@@ -3,13 +3,10 @@ import Modal.modal.models.kripke
 import Modal.modal.logics.logic_K
 
 
-open ModalFormula
-
-
 variable {α : Type}
 
 -- Soundness and completeness of logic K with respect to Kripke models
 -- Well-known result
 theorem logicK_kripke_sc :
-    ∀ (φ : ModalFormula α), Kripke.valid φ ↔ KProof φ := by
+    ∀ (φ : Modal.Formula α), Kripke.valid φ ↔ KProof φ := by
     admit
