Modal/modal/sound_complete/logicM_upnbhd.lean
@@ -3,7 +3,7 @@ import Modal.modal.models.nbhd
 import Modal.modal.logics.logic_M
 
 
-open ModalFormula Neighborhood
+open Neighborhood
 
 
 variable {α : Type}
@@ -11,5 +11,5 @@ variable {α : Type}
 -- Soundness and completeness of logic M with respect to upward-closed neighborhood models
 -- Well-known result - not specific to dual models
 theorem logicM_upnbhd_sc :
-    ∀ (φ : ModalFormula α), valid_in_class IsUpwardClosed φ ↔ MProof φ := by
+    ∀ (φ : Modal.Formula α), valid_in_class IsUpwardClosed φ ↔ MProof φ := by
     admit
